Prove UnionFind01

demo/union_find/UnionFind1.v
@@ -29,10 +29,11 @@ Definition f_new (oh0: owned_heap) (m0: mem) (vs0: list val):
   itree (E owned_heap) (owned_heap * (mem * val)) :=
   tau;;
   _ <- unwrapU (parg_new vs0) ;;
-  '(m1, b) <- unwrapU (malloc m0 (Ptrofs.repr 12)) ;;
+  '(m1, b) <- unwrapU (malloc m0 (Ptrofs.repr 16)) ;;
   let x  := Vptr b Ptrofs.zero in
-  m2 <- unwrapU (Mem.store Mptr m1 b 4 x) ;;
+  m2 <- unwrapU (Mem.store Mptr m1 b 8 x) ;;
   m3 <- unwrapU (Mem.store Mint32 m2 b 0 (Vint Int.zero)) ;;
+  tau;;
   Ret (oh0, (m3, x))
 .
 
@@ -44,39 +45,52 @@ Definition f_new (oh0: owned_heap) (m0: mem) (vs0: list val):
 
 Definition f_find (oh0: owned_heap) (m0: mem) (vs0: list val):
   itree (E owned_heap) (owned_heap * (mem * val)) :=
-  tau;;
   x <- unwrapU (parg_find vs0) ;;
-  p <- unwrapU (Mem.load Mptr m0 x 4) ;;
+  p <- unwrapU (Mem.load Mptr m0 x 8) ;;
   cond <- unwrapU (Val.cmplu_bool (Mem.valid_pointer m0) Cne p (Vptr x Ptrofs.zero)) ;;
+  tau;;
   myif (cond)
-    ('(oh1, (m1, p0)) <- trigger (ICall _find oh0 m0 [p]) ;; tau;;
-      m2 <- unwrapU (Mem.store Mptr m1 x 4 p0) ;;
+    (tau;; '(oh1, (m1, p0)) <- trigger (ICall _find oh0 m0 [p]) ;;
+      m2 <- unwrapU (Mem.store Mptr m1 x 8 p0) ;;
+      tau;;
       Ret (oh1, (m2, p0)))
-    (Ret (oh0, (m0, p)))
+    (tau;; Ret (oh0, (m0, p)))
+.
+
+Definition unint (v: val): option int :=
+  match v with
+  | Vint i => Some i
+  | _ => None
+  end
 .
 
 Definition f_union (oh0: owned_heap) (m0: mem) (vs0: list val):
   itree (E owned_heap) (owned_heap * (mem * val)) :=
-  tau;;
   '(x, y) <- unwrapU (parg_union vs0) ;;
+  tau;;
   '(oh1, (m1, xRoot)) <- trigger (ICall _find oh0 m0 [Vptr x Ptrofs.zero]) ;; tau;;
-  '(oh2, (m2, yRoot)) <- trigger (ICall _find oh0 m0 [Vptr x Ptrofs.zero]) ;; tau;;
+  '(oh2, (m2, yRoot)) <- trigger (ICall _find oh1 m1 [Vptr y Ptrofs.zero]) ;;
   cond <- unwrapU (Val.cmplu_bool (Mem.valid_pointer m2) Ceq xRoot yRoot) ;;
+  tau;;
   (myif cond
-        (Ret (oh2, (m2, Vundef)))
-        (` xRootB: block <- unwrapU (unblock xRoot) ;;
-         ` yRootB: block <- unwrapU (unblock yRoot) ;;
-         xRank <- unwrapU (Mem.load Mint32 m2 xRootB 0) ;;
-         yRank <- unwrapU (Mem.load Mint32 m2 yRootB 0) ;;
-         myif (Val.cmp_bool Clt xRank yRank)
-              (m3 <- unwrapU (Mem.store Mptr m2 xRootB 4 yRoot) ;;
-               Ret (oh2, (m3, Vundef)))
-              (myif (Val.cmp_bool Cgt xRank yRank)
-                    (m3 <- unwrapU (Mem.store Mptr m2 yRootB 4 xRoot) ;;
-                     Ret (oh2, (m3, Vundef)))
-                    (m3 <- unwrapU (Mem.store Mptr m2 yRootB 4 xRoot) ;;
-                     m4 <- unwrapU (Mem.store Mint32 m3 xRootB 0 (Val.add xRank (Vint Int.one))) ;;
-                     Ret (oh2, (m4, Vundef)))
+        (tau;; Ret (oh2, (m2, Vundef)))
+        (`xRootB: block <- unwrapU (unblock xRoot) ;;
+         `yRootB: block <- unwrapU (unblock yRoot) ;;
+         (* `xRank: int <- unwrapU (do _xRank <- Mem.load Mint32 m2 xRootB 0 ; (unint _xRank)) ;; *)
+         (* `yRank: int <- unwrapU (do _yRank <- Mem.load Mint32 m2 yRootB 0 ; (unint _yRank)) ;; *)
+         `_xRank: val <- unwrapU (Mem.load Mint32 m2 xRootB 0) ;;
+         `_yRank: val <- unwrapU (Mem.load Mint32 m2 yRootB 0) ;;
+         `xRank: int <- unwrapU (unint _xRank) ;;
+         `yRank: int <- unwrapU (unint _yRank) ;;
+         myif (Int.ltu xRank yRank)
+              (m3 <- unwrapU (Mem.store Mptr m2 xRootB 8 yRoot) ;;
+              tau;; Ret (oh2, (m3, Vundef)))
+              (myif (Int.ltu yRank xRank)
+                    (m3 <- unwrapU (Mem.store Mptr m2 yRootB 8 xRoot) ;;
+                     tau;; Ret (oh2, (m3, Vundef)))
+                    (m3 <- unwrapU (Mem.store Mptr m2 yRootB 8 xRoot) ;;
+                     m4 <- unwrapU (Mem.store Mint32 m3 xRootB 0 (Vint (Int.add xRank Int.one))) ;;
+                     tau;; Ret (oh2, (m4, Vundef)))
               )
         )
   )
