demo/union_find/UnionFind01proof.v
@@ -52,13 +52,28 @@ Proof.
   econs; ss; et.
   { ii. u. des_ifs. unfold internal_funs. des_ifs.
     Local Transparent build_composite_env'. (*** TODO: avoid this ***)
-    ss. exploit prog_defmap_image; et. ss. ii; des; ss.
+    exploit in_prog_defmap; et; intro T; ss; unfold update_snd in *; ss; des; clarify; ss.
     Local Opaque build_composite_env'.
   }
   ii.
   (*** THIS SHOULD BE PROVIDED FROM META THEORY ***)
-  assert(exists fblk, <<SYMB: Genv.find_symbol (geof skenv_link prog) _malloc = Some fblk>>).
+  assert(exists b_m, <<MSYMB: Genv.find_symbol (geof skenv_link prog) _malloc = Some b_m>>).
   {
+    inv INCL. ss.
+    exploit (DEFS _malloc); et.
+    { unfold prog_defmap. ss. }
+    i; des. ss. folder.
+    clear - SYMB.
+    Local Opaque PTree.get.
+    (*** TODO: Current: I can't use global opaque because of some extensional proofs. fix it ***)
+    uge. ss. rewrite MapsC.PTree_filter_key_spec. des_ifs. esplits; et.
+    Local Transparent PTree.get.
+  }
+  des.
+  (*** THIS SHOULD BE PROVIDED FROM META THEORY ***)
+  assert(exists b_n, <<NSYMB: Genv.find_symbol (geof skenv_link prog) _new = Some b_n>>).
+  {
+    clear_until TGT.
     inv INCL. ss.
     exploit (DEFS _new); et.
     { unfold prog_defmap. ss. }
@@ -71,10 +86,11 @@ Proof.
   }
   des.
   (*** THIS SHOULD BE PROVIDED FROM META THEORY ***)
-  assert(exists fblk, <<SYMB: Genv.find_symbol (geof skenv_link prog) _new = Some fblk>>).
+  assert(exists b_f, <<FSYMB: Genv.find_symbol (geof skenv_link prog) _find = Some b_f>>).
   {
+    clear_until TGT.
     inv INCL. ss.
-    exploit (DEFS _new); et.
+    exploit (DEFS _find); et.
     { unfold prog_defmap. ss. }
     i; des. ss. folder.
     clear - SYMB.
@@ -85,11 +101,52 @@ Proof.
   }
   des.
   (*** THIS SHOULD BE PROVIDED FROM META THEORY ***)
-  assert(FIBDEF: forall
+  assert(exists b_u, <<FSYMB: Genv.find_symbol (geof skenv_link prog) _union = Some b_u>>).
+  {
+    clear_until TGT.
+    inv INCL. ss.
+    exploit (DEFS _union); et.
+    { unfold prog_defmap. ss. }
+    i; des. ss. folder.
+    clear - SYMB.
+    Local Opaque PTree.get.
+    (*** TODO: Current: I can't use global opaque because of some extensional proofs. fix it ***)
+    uge. ss. rewrite MapsC.PTree_filter_key_spec. des_ifs. esplits; et.
+    Local Transparent PTree.get.
+  }
+  des.
+
+  (*** THIS SHOULD BE PROVIDED FROM META THEORY ***)
+  assert(_MDEF: forall
+            fblk
+            (SYMB: Genv.find_symbol (geof skenv_link prog) _malloc = Some fblk)
+          ,
+            <<NDEF: Genv.find_funct (geof skenv_link prog) (Vptr fblk Ptrofs.zero)
+                   = Some (Ctypes.External EF_malloc (Tcons tulong Tnil) (tptr tvoid) cc_default)>>).
+  { i.
+    exploit (SkEnv.project_impl_spec); try apply INCL. intro SPEC.
+    des. ss. des_ifs. clear_tac.
+    exploit CSkEnv.project_revive_precise; et. intro T. inv T.
+    exploit SYMB2P; et. intro U. dup U. unfold NW, defs in U0. des_sumbool.
+    exploit prog_defmap_dom; et. intro V; des.
+    exploit P2GE; et. intro W; des.
+    folder.
+    assert(b_m = b).
+    { clear - SPEC SYMB SYMB0 U. (*** TODO: this is too extensional ***) uge. ss. clarify. }
+    clarify.
+    Local Transparent build_composite_env'. (*** TODO: avoid this ***)
+    exploit (prog_defmap_norepet prog _malloc); ss; et.
+    { repeat (econs; ss; et; [ii; des; ss|]); repeat econs; ss; et. }
+    intro T. clarify. ss.
+    unfold Genv.find_funct_ptr. unfold Clight.fundef. rewrite DEF. ss.
+    Local Opaque build_composite_env'.
+  }
+  (*** THIS SHOULD BE PROVIDED FROM META THEORY ***)
+  assert(_NDEF: forall
             fblk
             (SYMB: Genv.find_symbol (geof skenv_link prog) _new = Some fblk)
           ,
-            <<DEF: Genv.find_funct (geof skenv_link prog) (Vptr fblk Ptrofs.zero)
+            <<NDEF: Genv.find_funct (geof skenv_link prog) (Vptr fblk Ptrofs.zero)
                    = Some (Ctypes.Internal f_new)>>).
   { i.
     exploit (SkEnv.project_impl_spec); try apply INCL. intro SPEC.
@@ -99,7 +156,7 @@ Proof.
     exploit prog_defmap_dom; et. intro V; des.
     exploit P2GE; et. intro W; des.
     folder.
-    assert(fblk = b).
+    assert(b_n = b).
     { clear - SPEC SYMB SYMB0 U. (*** TODO: this is too extensional ***) uge. ss. clarify. }
     clarify.
     Local Transparent build_composite_env'. (*** TODO: avoid this ***)
@@ -109,8 +166,73 @@ Proof.
     unfold Genv.find_funct_ptr. unfold Clight.fundef. rewrite DEF. ss.
     Local Opaque build_composite_env'.
   }
-  exploit FIBDEF; et. intro DEF. clear FIBDEF.
+  (*** THIS SHOULD BE PROVIDED FROM META THEORY ***)
+  assert(_FDEF: forall
+            fblk
+            (SYMB: Genv.find_symbol (geof skenv_link prog) _find = Some fblk)
+          ,
+            <<FDEF: Genv.find_funct (geof skenv_link prog) (Vptr fblk Ptrofs.zero)
+                   = Some (Ctypes.Internal f_find)>>).
+  { i.
+    exploit (SkEnv.project_impl_spec); try apply INCL. intro SPEC.
+    des. ss. des_ifs. clear_tac.
+    exploit CSkEnv.project_revive_precise; et. intro T. inv T.
+    exploit SYMB2P; et. intro U. dup U. unfold NW, defs in U0. des_sumbool.
+    exploit prog_defmap_dom; et. intro V; des.
+    exploit P2GE; et. intro W; des.
+    folder.
+    assert(b_f = b).
+    { clear - SPEC SYMB SYMB0 U. (*** TODO: this is too extensional ***) uge. ss. clarify. }
+    clarify.
+    Local Transparent build_composite_env'. (*** TODO: avoid this ***)
+    exploit (prog_defmap_norepet prog _find); ss; et.
+    { repeat (econs; ss; et; [ii; des; ss|]); repeat econs; ss; et. }
+    intro T. clarify. ss.
+    unfold Genv.find_funct_ptr. unfold Clight.fundef. rewrite DEF. ss.
+    Local Opaque build_composite_env'.
+  }
+  (*** THIS SHOULD BE PROVIDED FROM META THEORY ***)
+  assert(_UDEF: forall
+            fblk
+            (SYMB: Genv.find_symbol (geof skenv_link prog) _union = Some fblk)
+          ,
+            <<FDEF: Genv.find_funct (geof skenv_link prog) (Vptr fblk Ptrofs.zero)
+                   = Some (Ctypes.Internal f_union)>>).
+  { i.
+    exploit (SkEnv.project_impl_spec); try apply INCL. intro SPEC.
+    des. ss. des_ifs. clear_tac.
+    exploit CSkEnv.project_revive_precise; et. intro T. inv T.
+    exploit SYMB2P; et. intro U. dup U. unfold NW, defs in U0. des_sumbool.
+    exploit prog_defmap_dom; et. intro V; des.
+    exploit P2GE; et. intro W; des.
+    folder.
+    assert(b_u = b).
+    { clear - SPEC SYMB SYMB0 U. (*** TODO: this is too extensional ***) uge. ss. clarify. }
+    clarify.
+    Local Transparent build_composite_env'. (*** TODO: avoid this ***)
+    exploit (prog_defmap_norepet prog _union); ss; et.
+    { repeat (econs; ss; et; [ii; des; ss|]); repeat econs; ss; et. }
+    intro T. clarify. ss.
+    unfold Genv.find_funct_ptr. unfold Clight.fundef. rewrite DEF. ss.
+    Local Opaque build_composite_env'.
+  }
+
+  exploit _MDEF; et. intro MDEF. clear _MDEF.
+  exploit _NDEF; et. intro NDEF. clear _NDEF.
+  exploit _FDEF; et. intro FDEF. clear _FDEF.
+  exploit _UDEF; et. intro UDEF. clear _UDEF.
   des.
+
+  ss. des_ifs. clear_tac.
+  (* hexploit (prog_comp_env_eq prog); et. intro CE. *)
+  (* hexploit build_composite_env_consistent; et. intro CEC. *)
+  (*** above (CEC) will prevent future des_ifs, dependent type thing ***)
+  (* exploit (CEC _Node); et. *)
+  (* { ss. } *)
+  (* intro V. inv V. ss. des_ifs. clear_tac. *)
+  (*** it seems CEC is actually not that useful here --
+       local transparent blah && extensional proof do the thing ***)
+
 
 
   exploit prog_defmap_image; et. ss. des_ifs.
@@ -144,177 +266,436 @@ Proof.
       { econs; ss; et.
         - econs; ss; et.
           + econsby ss; et.
+          + econsby ss; et.
+        - repeat econs; ss; et.
       }
       apply star_refl.
-      des_ifs.
-      
+    }
+
+    rewrite bind_ret_l. left. pfold.
+    unfold unwrapU, malloc. uo. des_ifs; cycle 1.
+    { unfold triggerUB. irw. econs; ss; et. }
+    ss. rewrite bind_ret_l. des_ifs; cycle 1.
+    { unfold triggerUB. irw. econs; ss; et. }
+    rewrite bind_ret_l. des_ifs; cycle 1.
+    { unfold triggerUB. irw. econs; ss; et. }
+    rewrite bind_ret_l.
+
+    assert(SZ: co_sizeof c = 16).
+    {
+      Local Transparent build_composite_env'. (*** TODO: avoid this ***)
+      cbn in Heq3.
+      Local Opaque build_composite_env'.
+      clarify.
+    }
+    assert(MEM: co_members c = [(_rank, tuint); (_parent, tptr (Tstruct _Node noattr))]).
+    {
+      Local Transparent build_composite_env'. (*** TODO: avoid this ***)
+      cbn in Heq3.
+      Local Opaque build_composite_env'.
+      clarify.
+    }
+    assert(ALN: co_alignof c =  8).
+    {
+      Local Transparent build_composite_env'. (*** TODO: avoid this ***)
+      cbn in Heq3.
+      Local Opaque build_composite_env'.
+      clarify.
+    }
+
+    econs; ss; et; cycle 1.
+    { eapply plus_left with (t1 := E0) (t2 := E0); ss.
+      { econsr; ss; et. econs; ss; et.
+        { unfold Mptr. des_ifs; ss. rewrite SZ; et. }
+        { unfold Mptr. des_ifs; ss. rewrite SZ; et. }
+      }
+      eapply star_left with (t1 := E0) (t2 := E0); ss.
+      { _step. }
+      eapply star_left with (t1 := E0) (t2 := E0); ss.
+      { _step. }
+      eapply star_left with (t1 := E0) (t2 := E0); ss.
+      { _step. }
+      eapply star_left with (t1 := E0) (t2 := E0); ss.
+      { _step. }
+      eapply star_left with (t1 := E0) (t2 := E0); ss.
+      { _step. }
+      eapply star_left with (t1 := E0) (t2 := E0); ss.
+      { econs; ss; et.
+        - econs; ss; et.
+          + _step.
+          + rewrite MEM. ss.
+        - repeat econs; ss; et.
+        - repeat econs; ss; et.
+        - repeat econs; ss; et.
+      }
+      eapply star_left with (t1 := E0) (t2 := E0); ss.
+      { _step. }
+      eapply star_left with (t1 := E0) (t2 := E0); ss.
+      { _step. }
+      eapply star_left with (t1 := E0) (t2 := E0); ss.
+      { econs; ss; et.
+        - econs; ss; et.
+          + _step.
+          + rewrite MEM. ss.
+        - repeat econs; ss; et.
+        - repeat econs; ss; et.
+        - repeat econs; ss; et.
+      }
+      eapply star_left with (t1 := E0) (t2 := E0); ss.
+      { _step. }
       eapply star_left with (t1 := E0) (t2 := E0); ss.
       { _step. }
       apply star_refl.
     }
+    left. pfold. econs; ss; et.
+    econs; ss; et.
 
-    destruct (classic (Int.eq n Int.zero)).
-    { apply_all_once Int.same_if_eq. clarify.
-      pfold. econs; ss; et; cycle 1.
-      { eapply plus_left with (t1 := E0) (t2 := E0); ss.
-        { _step. }
-        eapply star_left with (t1 := E0) (t2 := E0); ss.
-        { _step. }
-        des_ifs.
-        eapply star_left with (t1 := E0) (t2 := E0); ss.
-        { _step. }
-        apply star_refl.
-      }
-      { des_ifs. left. pfold. econs; ss; et. econs; ss; et. }
-    }
-    rename H into NZERO.
-    destruct (classic (Int.eq n Int.one)).
-    { apply_all_once Int.same_if_eq. clarify.
-      pfold. econs; ss; et; cycle 1.
-      { eapply plus_left with (t1 := E0) (t2 := E0); ss.
-        { _step. }
-        eapply star_left with (t1 := E0) (t2 := E0); ss.
-        { _step. }
-        des_ifs.
-        eapply star_left with (t1 := E0) (t2 := E0); ss.
-        { _step. }
-        eapply star_left with (t1 := E0) (t2 := E0); ss.
-        { _step. }
-        eapply star_left with (t1 := E0) (t2 := E0); ss.
-        { _step. }
-        eapply star_left with (t1 := E0) (t2 := E0); ss.
-        { _step. }
-        apply star_refl.
-      }
-      { des_ifs. left. pfold. econs; ss; et. econs; ss; et. }
-    }
-    rename H into NONE.
-
+  -
+    exploit (prog_defmap_norepet prog _find); et.
+    { repeat (econs; ss; et); ii; des; ss. }
     {
+      Local Transparent build_composite_env'. (*** TODO: avoid this ***)
+      ss; et.
+      Local Opaque build_composite_env'.
+    }
+    ii; clarify. cbn in SRC. des_ifs. clear_tac.
+    econs; ss; et. ii. inv TYP. ss. destruct vs0; ss. destruct vs0; ss.
+    unfold typify_list, typify in TYP0. ss. des_ifs; ss. clear_tac.
+
+    esplits; et.
+    {
+      Local Transparent build_composite_env'. (*** TODO: avoid this ***)
+      repeat (econs; ss; et).
+      _step.
+      Local Opaque build_composite_env'.
+    }
+    unfold UnionFind1.f_find. ss.
+    destruct (unblock v) eqn:T; cycle 1.
+    { ss. pfold. unfold triggerUB. irw. econs; ss; et. }
+    destruct v; ss. des_ifs. clear_tac.
+    irw. unfold unwrapU. des_ifs; cycle 1.
+    { ss. pfold. unfold triggerUB. irw. econs; ss; et. }
+    irw.
+    des_ifs; cycle 1.
+    { ss. pfold. unfold triggerUB. irw. econs; ss; et. }
+    irw.
+    pfold. econs; ss; et; cycle 1.
+    { eapply plus_left with (t1 := E0) (t2 := E0); ss.
+      { _step. }
+      eapply star_left with (t1 := E0) (t2 := E0); ss.
+      { _step. }
+      (* { repeat (first[econsby ss; et|econs; ss; et]). } *) (*** TODO: <--- make this as a tactic ***)
+      eapply star_left with (t1 := E0) (t2 := E0); ss.
+      { _step. }
+      eapply star_left with (t1 := E0) (t2 := E0); ss.
+      { _step. }
+      apply star_refl.
+    }
+    destruct b0; ss.
+    + left. pfold. econs; ss; et; cycle 1.
+      { eapply plus_left with (t1 := E0) (t2 := E0); ss.
+        { repeat (econs; ss; et).
+          - cbn. unfold Cop.cmp_ptr. des_ifs. unfold option_map. des_ifs.
+          - ss.
+        }
+        eapply star_left with (t1 := E0) (t2 := E0); ss.
+        { _step. }
+        eapply star_left with (t1 := E0) (t2 := E0); ss.
+        { _step. }
+        eapply star_left with (t1 := E0) (t2 := E0); ss.
+        { repeat (first[econsby ss; et|econs; ss; et]). (*** TODO: <--- make this as a tactic ***)
+          cbn. des_ifs.
+        }
+        apply star_refl.
+      }
+      left. pfold. econs; ss; et.
+      { econs; ss; et. clear_tac. clear - Heq0. cbn. unfold typify. destruct v; ss.
+        - des_ifs_safe. ss. des_ifs.
+        - des_ifs_safe. ss. des_ifs.
+      }
+      { econs; ss; et. ii; clarify. }
+      ii. left. pfold.
+      des_ifs; cycle 1.
+      { unfold triggerUB. irw. econs; ss; et. }
+      irw.
+      econs; ss; et; cycle 1.
+      { eapply plus_left with (t1 := E0) (t2 := E0); ss.
+        { _step. }
+        eapply star_left with (t1 := E0) (t2 := E0); ss.
+        { _step. }
+        eapply star_left with (t1 := E0) (t2 := E0); ss.
+        { _step. }
+        eapply star_left with (t1 := E0) (t2 := E0); ss.
+        { _step. }
+        eapply star_left with (t1 := E0) (t2 := E0); ss.
+        { _step. }
+        eapply star_left with (t1 := E0) (t2 := E0); ss.
+        { _step. }
+        eapply star_left with (t1 := E0) (t2 := E0); ss.
+        { repeat (first[econsby ss; et|econs; ss; et]). (*** TODO: <--- make this as a tactic ***)
+          - rewrite Cop.cast_val_casted; ss.
+        }
+        eapply star_left with (t1 := E0) (t2 := E0); ss.
+        { _step. }
+        eapply star_left with (t1 := E0) (t2 := E0); ss.
+        { repeat (first[econsby ss; et|econs; ss; et]). (*** TODO: <--- make this as a tactic ***)
+          - rewrite Cop.cast_val_casted; ss.
+        }
+        apply star_refl.
+      }
+      left. pfold. econs; ss; et.
+    + left. pfold. econs; ss; et; cycle 1.
+      { eapply plus_left with (t1 := E0) (t2 := E0); ss.
+        { repeat (econs; ss; et).
+          - cbn. unfold Cop.cmp_ptr. des_ifs. unfold option_map. des_ifs.
+          - ss.
+        }
+        eapply star_left with (t1 := E0) (t2 := E0); ss.
+        { _step. }
+        eapply star_left with (t1 := E0) (t2 := E0); ss.
+        { repeat (first[econsby ss; et|econs; ss; et]). (*** TODO: <--- make this as a tactic ***)
+          cbn. des_ifs.
+        }
+        apply star_refl.
+      }
+      left. pfold. econs; ss; et.
+      { destruct v; ss.
+        - econs; ss; et.
+        - econs; ss; et.
+      }
+
+  -
+    exploit (prog_defmap_norepet prog _union); et.
+    { repeat (econs; ss; et); ii; des; ss. }
+    {
+      Local Transparent build_composite_env'. (*** TODO: avoid this ***)
+      ss; et.
+      Local Opaque build_composite_env'.
+    }
+    ii; clarify. cbn in SRC. des_ifs. clear_tac.
+    econs; ss; et. ii. inv TYP. ss. destruct vs0; ss. destruct vs0; ss. destruct vs0; ss.
+    unfold typify_list, typify in TYP0. ss. des_ifs; ss. clear_tac.
+
+    esplits; et.
+    {
+      Local Transparent build_composite_env'. (*** TODO: avoid this ***)
+      repeat (econs; ss; et).
+      { ii; des; ss. }
+      _step.
+      Local Opaque build_composite_env'.
+    }
+    rename v into vx. rename v0 into vy.
+    unfold UnionFind1.f_union. ss.
+    destruct (unblock vx) eqn:BX; cycle 1.
+    { ss. pfold. unfold triggerUB. irw. econs; ss; et. }
+    destruct (unblock vy) eqn:BY; cycle 1.
+    { ss. pfold. unfold triggerUB. irw. econs; ss; et. }
+    destruct vx; ss. destruct vy; ss. des_ifs.
+    rename b into b_x. rename b0 into b_y.
+    irw. pfold. econs; ss; et; cycle 1.
+    { eapply plus_left with (t1 := E0) (t2 := E0); ss.
+      { _step. }
+      eapply star_left with (t1 := E0) (t2 := E0); ss.
+      { _step. }
+      eapply star_left with (t1 := E0) (t2 := E0); ss.
+      { _step. }
+      apply star_refl.
+    }
+    left. pfold. econs; ss; et.
+    { econs; ss; et. cbn. unfold typify. des_ifs. }
+    { econs; ss; et. }
+    ii.
+    left. pfold. econs; ss; et; cycle 1.
+    { eapply plus_left with (t1 := E0) (t2 := E0); ss.
+      { _step. }
+      eapply star_left with (t1 := E0) (t2 := E0); ss.
+      { _step. }
+      eapply star_left with (t1 := E0) (t2 := E0); ss.
+      { _step. }
+      eapply star_left with (t1 := E0) (t2 := E0); ss.
+      { _step. }
+      eapply star_left with (t1 := E0) (t2 := E0); ss.
+      { _step. }
+      eapply star_left with (t1 := E0) (t2 := E0); ss.
+      { repeat (first[econsby ss; et|econs; ss; et]). (*** TODO: <--- make this as a tactic ***) }
+      apply star_refl.
+    }
+    left. pfold. irw. econs; ss; et.
+    { econs; ss; et. cbn. unfold typify. des_ifs. }
+    { econs; ss; et. }
+    ii. left.
+    destruct (Val.cmplu_bool (Mem.valid_pointer m2) Ceq v1 v0) eqn:T; cycle 1.
+    { ss. pfold. unfold triggerUB. irw. econs; ss; et. }
+    ss. irw.
+    pfold. econs; ss; et; cycle 1.
+    { eapply plus_left with (t1 := E0) (t2 := E0); ss.
+      { _step. }
+      eapply star_left with (t1 := E0) (t2 := E0); ss.
+      { _step. }
+      eapply star_left with (t1 := E0) (t2 := E0); ss.
+      { _step. }
+      eapply star_left with (t1 := E0) (t2 := E0); ss.
+      { _step. }
+      apply star_refl.
+    }
+    left.
+    destruct b.
+    { cbn.
       pfold. econs; ss; et; cycle 1.
       { eapply plus_left with (t1 := E0) (t2 := E0); ss.
-        { _step. }
-        eapply star_left with (t1 := E0) (t2 := E0); ss.
-        { repeat (econs; ss; et). ss. rewrite Int.eq_false; ss. ii; clarify. }
-        eapply star_left with (t1 := E0) (t2 := E0); ss.
-        { _step. }
-        eapply star_left with (t1 := E0) (t2 := E0); ss.
-        { _step. }
-        eapply star_left with (t1 := E0) (t2 := E0); ss.
-        { repeat (econs; ss; et). ss. rewrite Int.eq_false; ss. ii; clarify. }
-        eapply star_left with (t1 := E0) (t2 := E0); ss.
-        { _step. }
-        eapply star_left with (t1 := E0) (t2 := E0); ss.
-        { _step. }
-        eapply star_left with (t1 := E0) (t2 := E0); ss.
-        { _step. }
+        { repeat (econs; ss; et).
+          - cbn. unfold Cop.cmp_ptr. des_ifs. unfold option_map. des_ifs.
+          - ss.
+        }
         eapply star_left with (t1 := E0) (t2 := E0); ss.
         { _step. }
         apply star_refl.
       }
-      des_ifs. rewrite bind_trigger.
-      left. pfold. econs; ss; et.
-      { econs; ss; et. cbn. unfold typify. des_ifs; ss. }
-      { econs; ss. }
-      ii.
-      left. pfold. econs; ss; et; cycle 1.
-      { eapply plus_left with (t1 := E0) (t2 := E0); ss.
-        { _step. }
-        eapply star_left with (t1 := E0) (t2 := E0); ss.
-        { _step. }
-        eapply star_left with (t1 := E0) (t2 := E0); ss.
-        { _step. }
-        eapply star_left with (t1 := E0) (t2 := E0); ss.
-        { _step. }
-        eapply star_left with (t1 := E0) (t2 := E0); ss.
-        { _step. }
-        eapply star_left with (t1 := E0) (t2 := E0); ss.
-        { _step. }
-        apply star_refl.
-      }
-      left. pfold.
-      rewrite bind_trigger.
-      econs; ss; et.
-      { econs; ss; et. cbn. unfold typify. des_ifs; ss. }
-      { econs; ss; et. }
-      ii. inv TYP; ss. inv TYP0; ss. clear_tac.
-      left. pfold. econs; ss; et; cycle 1.
-      { eapply plus_left with (t1 := E0) (t2 := E0); ss.
-        { _step. }
-        eapply star_left with (t1 := E0) (t2 := E0); ss.
-        { _step. }
-        eapply star_left with (t1 := E0) (t2 := E0); ss.
-        { _step. }
-        eapply star_left with (t1 := E0) (t2 := E0); ss.
-        { _step. }
-        apply star_refl.
-      }
-      { left. pfold. econs; ss; et. econs; ss; et. }
+      ss. left. pfold. econs; ss; et.
+      { econs; et. }
     }
+    cbn.
+    destruct (unblock v1) eqn:BX; cycle 1.
+    { ss. pfold. unfold triggerUB. irw. econs; ss; et. }
+    destruct (unblock v0) eqn:BY; cycle 1.
+    { ss. pfold. unfold triggerUB. irw. econs; ss; et. }
+    ss. irw.
+    destruct (Mem.load Mint32 m2 b 0) eqn:LX; cycle 1.
+    { ss. pfold. unfold triggerUB. irw. econs; ss; et. }
+    destruct (Mem.load Mint32 m2 b0 0) eqn:LY; cycle 1.
+    { ss. pfold. unfold triggerUB. irw. econs; ss; et. }
+    ss. irw.
+    Local Opaque Val.cmplu_bool.
+    destruct v1; ss. destruct v0; ss. des_ifs_safe. rename b into b_x0. rename b0 into b_y0.
+    rename v into _xRank. rename v2 into _yRank.
+    destruct (unint _xRank) eqn:IX; cycle 1.
+    { ss. pfold. unfold triggerUB. irw. econs; ss; et. }
+    destruct (unint _yRank) eqn:IY; cycle 1.
+    { ss. pfold. unfold triggerUB. irw. econs; ss; et. }
+    destruct _xRank, _yRank; ss. clarify.
+    rename i into xRank. rename i0 into yRank.
+    irw.
+
+    destruct (Int.ltu xRank yRank) eqn:C0; ss.
+    { destruct (Mem.store Mptr m2 b_x0 8 (Vptr b_y0 Ptrofs.zero)) eqn:S; cycle 1.
+      { ss. pfold. unfold triggerUB. irw. econs; ss; et. }
+      ss. irw. pfold. econs; ss; et; cycle 1.
+      { eapply plus_left with (t1 := E0) (t2 := E0); ss.
+        { repeat (econs; ss; et).
+          - cbn. unfold Cop.cmp_ptr. des_ifs. unfold option_map. des_ifs.
+          - ss.
+        }
+        eapply star_left with (t1 := E0) (t2 := E0); ss.
+        { _step. }
+        eapply star_left with (t1 := E0) (t2 := E0); ss.
+        { _step. }
+        eapply star_left with (t1 := E0) (t2 := E0); ss.
+        { repeat (first[econsby ss; et|econs; ss; et]). }
+        eapply star_left with (t1 := E0) (t2 := E0); ss.
+        { _step. }
+        eapply star_left with (t1 := E0) (t2 := E0); ss.
+        { _step. }
+        eapply star_left with (t1 := E0) (t2 := E0); ss.
+        { _step. }
+        eapply star_left with (t1 := E0) (t2 := E0); ss.
+        { _step. }
+        eapply star_left with (t1 := E0) (t2 := E0); ss.
+        { repeat (first[econsby ss; et|econs; ss; et]). cbn. des_ifs. }
+        eapply star_left with (t1 := E0) (t2 := E0); ss.
+        { cbn. rewrite Int.eq_false; ss.
+          repeat (first[econsby ss; et|econs; ss; et]).
+        }
+        eapply star_left with (t1 := E0) (t2 := E0); ss.
+        { _step. }
+        apply star_refl.
+      }
+      left. pfold. econs; ss; et.
+      { econs; ss; et. }
+    }
+    destruct (Int.ltu yRank xRank) eqn:C1; ss.
+    { destruct (Mem.store Mptr m2 b_y0 8 (Vptr b_x0 Ptrofs.zero)) eqn:S; cycle 1.
+      { ss. pfold. unfold triggerUB. irw. econs; ss; et. }
+      ss. irw. pfold. econs; ss; et; cycle 1.
+      { eapply plus_left with (t1 := E0) (t2 := E0); ss.
+        { repeat (econs; ss; et).
+          - cbn. unfold Cop.cmp_ptr. des_ifs. unfold option_map. des_ifs.
+          - ss.
+        }
+        eapply star_left with (t1 := E0) (t2 := E0); ss.
+        { _step. }
+        eapply star_left with (t1 := E0) (t2 := E0); ss.
+        { _step. }
+        eapply star_left with (t1 := E0) (t2 := E0); ss.
+        { repeat (first[econsby ss; et|econs; ss; et]). }
+        eapply star_left with (t1 := E0) (t2 := E0); ss.
+        { _step. }
+        eapply star_left with (t1 := E0) (t2 := E0); ss.
+        { _step. }
+        eapply star_left with (t1 := E0) (t2 := E0); ss.
+        { _step. }
+        eapply star_left with (t1 := E0) (t2 := E0); ss.
+        { _step. }
+        eapply star_left with (t1 := E0) (t2 := E0); ss.
+        { repeat (first[econsby ss; et|econs; ss; et]). cbn. des_ifs. }
+        eapply star_left with (t1 := E0) (t2 := E0); ss.
+        { cbn. rewrite Int.eq_true; ss.
+          repeat (first[econsby ss; et|econs; ss; et]).
+          cbn. des_ifs.
+        }
+        eapply star_left with (t1 := E0) (t2 := E0); ss.
+        { _step. }
+        eapply star_left with (t1 := E0) (t2 := E0); ss.
+        { _step. }
+        apply star_refl.
+      }
+      left. pfold. econs; ss; et.
+      { econs; ss; et. }
+    }
+    destruct (Mem.store Mptr m2 b_y0 8 (Vptr b_x0 Ptrofs.zero)) eqn:S0; cycle 1.
+    { ss. pfold. unfold triggerUB. irw. econs; ss; et. }
+    ss. irw.
+    destruct (Mem.store Mint32 m b_x0 0 (Vint (Int.add xRank Int.one))) eqn:S1; cycle 1.
+    { ss. pfold. unfold triggerUB. irw. econs; ss; et. }
+    ss. irw.
+    pfold. econs; ss; et; cycle 1.
+    { eapply plus_left with (t1 := E0) (t2 := E0); ss.
+      { repeat (econs; ss; et).
+        - cbn. unfold Cop.cmp_ptr. des_ifs. unfold option_map. des_ifs.
+        - ss.
+      }
+      eapply star_left with (t1 := E0) (t2 := E0); ss.
+      { _step. }
+      eapply star_left with (t1 := E0) (t2 := E0); ss.
+      { _step. }
+      eapply star_left with (t1 := E0) (t2 := E0); ss.
+      { repeat (first[econsby ss; et|econs; ss; et]). }
+      eapply star_left with (t1 := E0) (t2 := E0); ss.
+      { _step. }
+      eapply star_left with (t1 := E0) (t2 := E0); ss.
+      { _step. }
+      eapply star_left with (t1 := E0) (t2 := E0); ss.
+      { _step. }
+      eapply star_left with (t1 := E0) (t2 := E0); ss.
+      { _step. }
+      eapply star_left with (t1 := E0) (t2 := E0); ss.
+      { repeat (first[econsby ss; et|econs; ss; et]). cbn. des_ifs. }
+      eapply star_left with (t1 := E0) (t2 := E0); ss.
+      { cbn. rewrite Int.eq_true; ss.
+        repeat (first[econsby ss; et|econs; ss; et]).
+        cbn. des_ifs.
+      }
+      eapply star_left with (t1 := E0) (t2 := E0); ss.
+      { _step. }
+      eapply star_left with (t1 := E0) (t2 := E0); ss.
+      { _step. }
+      eapply star_left with (t1 := E0) (t2 := E0); ss.
+      { _step. }
+      eapply star_left with (t1 := E0) (t2 := E0); ss.
+      { _step. }
+      eapply star_left with (t1 := E0) (t2 := E0); ss.
+      { _step. }
+      apply star_refl.
+    }
+    left. pfold. econs; ss; et.
+    { econs; ss; et. }
 Qed.
-
-
-
-(* Section SIMMODSEM. *)
-
-(* Variable skenv_link: SkEnv.t. *)
-(* Variable sm_link: SimMem.t. *)
-(* Let md_src: Mod.t := (UnionFind1.module). *)
-(* Let md_tgt: Mod.t := (UnionFind0.module). *)
-(* Hypothesis (INCL: SkEnv.includes skenv_link (Mod.sk md_src)). *)
-(* (* Let INCLTGT: SkEnv.includes skenv_link (Mod.sk md_tgt). *) *)
-(* (* Proof. ss. Qed. *) *)
-(* Hypothesis (WF: SkEnv.wf skenv_link). *)
-(* Let ge := (SkEnv.project skenv_link (Mod.sk md_src)). *)
-(* Let tge := Build_genv (SkEnv.revive (SkEnv.project skenv_link (Mod.sk md_tgt)) prog) prog.(prog_comp_env). *)
-(* Definition msp: ModSemPair.t := *)
-(*   ModSemPair.mk (md_src skenv_link) (md_tgt skenv_link) (SimSymbId.mk md_src md_tgt) sm_link. *)
-
-(* Global Opaque _fib. *)
-(* Lemma unsymb *)
-(*       fid fblk *)
-(*       (FID: Genv.find_symbol ge fid = Some fblk) *)
-(*   : *)
-(*     <<FID: fid = _fib>> *)
-(* . *)
-(* Proof. *)
-(*   subst ge. ss. uge. ss. rewrite MapsC.PTree_filter_key_spec in *. des_ifs. *)
-(*   unfold defs in *. des_sumbool. ss. des; ss. *)
-(* Qed. *)
-
-(* Lemma symb_fib *)
-(*   : *)
-(*     exists fblk, <<FID: Genv.find_symbol tge _fib = Some fblk>> *)
-(* . *)
-(* Proof. *)
-(*   inv INCL. ss. *)
-(*   exploit (DEFS _fib); et. *)
-(*   { unfold prog_defmap. ss. } *)
-(*   i; des. ss. folder. *)
-(*   clear - SYMB. *)
-(*   subst ge. ss. uge. ss. rewrite MapsC.PTree_filter_key_spec. des_ifs. et. *)
-(* Qed. *)
-
-(* Lemma fib_def *)
-(*       fblk *)
-(*       (SYMB: Genv.find_symbol ge _fib = Some fblk) *)
-(*   : *)
-(*     <<DEF: Genv.find_funct tge (Vptr fblk Ptrofs.zero) = Some (Ctypes.Internal f_fib)>> *)
-(* . *)
-(* Proof. *)
-(*   exploit (SkEnv.project_impl_spec); try apply INCL. intro SPEC. *)
-(*   des. subst tge. ss. des_ifs. clear_tac. *)
-(*   exploit CSkEnv.project_revive_precise; et. intro T. inv T. *)
-(*   exploit SYMB2P; et. intro U. dup U. unfold NW, defs in U0. des_sumbool. *)
-(*   exploit prog_defmap_dom; et. intro V; des. *)
-(*   exploit P2GE; et. intro W; des. *)
-(*   folder. *)
-(*   assert(fblk = b). *)
-(*   { clear - SPEC SYMB SYMB0 U. (*** TODO: this is too extensional ***) uge. ss. clarify. } *)
-(*   clarify. *)
-(*   exploit (prog_defmap_norepet prog _fib); ss; et. *)
-(*   { repeat (econs; ss; et; [ii; des; ss|]); repeat econs; ss; et. } *)
-(*   intro T. clarify. ss. *)
-(*   unfold Genv.find_funct_ptr. unfold Clight.fundef. rewrite DEF. ss. *)
-(* Qed. *)
-
